Codegen.thy
@@ -74,7 +74,8 @@ fun OrderDAG_Int::  "(integer, integer\<times>integer) pre_digraph \<Rightarrow>
  integer \<Rightarrow> (integer set \<times> integer list)" 
  where " OrderDAG_Int V a =  (OrderDAG V (nat_of_integer a))"
 
-export_code anticone set blockDAG pre_digraph_ext snd fst vote_Spectre_Int SpectreOrder_Int OrderDAG_Int
+export_code top_sort anticone set blockDAG pre_digraph_ext snd fst vote_Spectre_Int
+ SpectreOrder_Int OrderDAG_Int
  in Haskell module_name DAGS file "code/" 
 
 end
